prove env call typing soundness

rocq/theories/TypeSystem/EnvTypingSoundness.v
@@ -42,6 +42,116 @@ Proof.
       exists st0. simpl. rewrite Hname. split; assumption.
 Qed.
 
+Fixpoint call_expr (e : expr) : bool :=
+  match e with
+  | EUnit => true
+  | ELit _ => true
+  | EVar _ => true
+  | EFn _ => true
+  | EPlace _ => true
+  | ELet _ _ _ e1 e2 => call_expr e1 && call_expr e2
+  | ELetInfer _ _ e1 e2 => call_expr e1 && call_expr e2
+  | ECall _ args => forallb call_expr args
+  | ECallExpr callee args => call_expr callee && forallb call_expr args
+  | EDeref e1 => call_expr e1
+  | EDrop e1 => call_expr e1
+  | EIf e1 e2 e3 => call_expr e1 && call_expr e2 && call_expr e3
+  | EStruct _ _ _ _ => false
+  | EReplace _ _ => false
+  | EAssign _ _ => false
+  | EBorrow _ _ => false
+  end.
+
+Definition call_exprs (args : list expr) : bool := forallb call_expr args.
+
+Lemma call_exprs_in_true :
+  forall args e,
+    call_exprs args = true ->
+    In e args ->
+    call_expr e = true.
+Proof.
+  unfold call_exprs.
+  intros args e Hargs Hin.
+  rewrite forallb_forall in Hargs.
+  apply Hargs. exact Hin.
+Qed.
+
+Fixpoint infer_env_args_collect fuel env Ω n (Σ : sctx) (args : list expr)
+    : infer_result (list Ty * sctx) :=
+  match args with
+  | [] => infer_ok ([], Σ)
+  | e :: rest =>
+      match infer_core_env_state_fuel fuel env Ω n Σ e with
+      | infer_err err => infer_err err
+      | infer_ok (T_e, Σ1) =>
+          match infer_env_args_collect fuel env Ω n Σ1 rest with
+          | infer_err err => infer_err err
+          | infer_ok (tys, Σ2) => infer_ok (T_e :: tys, Σ2)
+          end
+      end
+  end.
+
+Lemma infer_env_args_collect_eq :
+  forall fuel env Ω n args Σ,
+    (fix collect (Σ0 : sctx) (as_ : list expr) : infer_result (list Ty * sctx) :=
+       match as_ with
+       | [] => infer_ok ([], Σ0)
+       | e' :: es =>
+           match infer_core_env_state_fuel fuel env Ω n Σ0 e' with
+           | infer_err err => infer_err err
+           | infer_ok (T_e, Σ1) =>
+               match collect Σ1 es with
+               | infer_err err => infer_err err
+               | infer_ok (tys, Σ2) => infer_ok (T_e :: tys, Σ2)
+               end
+           end
+       end) Σ args =
+    infer_env_args_collect fuel env Ω n Σ args.
+Proof.
+  intros fuel env Ω n args.
+  induction args as [|e rest IH]; intros Σ; simpl.
+  - reflexivity.
+  - destruct (infer_core_env_state_fuel fuel env Ω n Σ e) as [[T_e Σ1] | err] eqn:He;
+      [rewrite IH |]; reflexivity.
+Qed.
+
+Lemma infer_env_args_collect_sound :
+  forall fuel env Ω n Σ args arg_tys params Σ',
+    infer_env_args_collect fuel env Ω n Σ args = infer_ok (arg_tys, Σ') ->
+    (forall Σ0 e T Σ1,
+        In e args ->
+        infer_core_env_state_fuel fuel env Ω n Σ0 e = infer_ok (T, Σ1) ->
+        typed_env_structural env Ω n Σ0 e T Σ1) ->
+    check_args Ω arg_tys params = None ->
+    typed_args_env_structural env Ω n Σ args params Σ'.
+Proof.
+  intros fuel env Ω n Σ args.
+  revert Σ.
+  induction args as [|e rest IH]; intros Σ arg_tys params Σ' Hcollect Hexpr Hcheck.
+  - simpl in Hcollect. inversion Hcollect; subst.
+    destruct params; simpl in Hcheck; [constructor | discriminate].
+  - simpl in Hcollect.
+    destruct (infer_core_env_state_fuel fuel env Ω n Σ e) as [[T_e Σ1] | err] eqn:He;
+      try discriminate.
+    destruct (infer_env_args_collect fuel env Ω n Σ1 rest) as [[tys Σ2] | err'] eqn:Htail;
+      try discriminate.
+    inversion Hcollect; subst.
+    destruct params as [|p ps]; simpl in Hcheck; try discriminate.
+    destruct (ty_compatible_b Ω T_e (param_ty p)) eqn:Hcompat; try discriminate.
+    eapply TESArgs_Cons.
+    + eapply Hexpr.
+      * left. reflexivity.
+      * exact He.
+    + exact Hcompat.
+    + eapply IH.
+      * exact Htail.
+      * intros Σ0 e0 T0 Σ0' Hin Hinfer0.
+        eapply Hexpr.
+        -- right. exact Hin.
+        -- exact Hinfer0.
+      * exact Hcheck.
+Qed.
+
 Lemma sctx_path_available_success :
   forall Σ x path,
     sctx_path_available Σ x path = infer_ok tt ->
@@ -302,6 +412,200 @@ Proof.
       * apply ty_core_eqb_true. exact Hbool.
       * eapply IH; [exact Hbasic2 | exact He2].
       * eapply IH; [exact Hbasic3 | exact He3].
+      * apply ty_core_eqb_true. exact Hcore.
+      * exact Hmerge.
+Qed.
+
+Theorem infer_core_env_state_fuel_call_structural_sound :
+  forall fuel env Ω n Σ e T Σ',
+    call_expr e = true ->
+    infer_core_env_state_fuel fuel env Ω n Σ e = infer_ok (T, Σ') ->
+    typed_env_structural env Ω n Σ e T Σ'.
+Proof.
+  induction fuel as [| fuel' IH]; intros env Ω n Σ e T Σ' Hcall Hinfer.
+  - simpl in Hinfer. discriminate.
+  - destruct e; simpl in Hcall; simpl in Hinfer; try discriminate.
+    + inversion Hinfer; subst. constructor.
+    + destruct l; inversion Hinfer; subst; constructor.
+    + destruct (sctx_lookup i Σ) as [[Tvar st] |] eqn:Hlookup; try discriminate.
+      destruct (binding_available_b st []) eqn:Havailable; try discriminate.
+      destruct (consume_place_value env Σ (PVar i) Tvar) as [Σ0 | err] eqn:Hconsume;
+        try discriminate.
+      unfold consume_place_value in Hconsume.
+      destruct (usage_eqb (ty_usage Tvar) UUnrestricted) eqn:Husage.
+      * inversion Hconsume; subst.
+        inversion Hinfer; subst.
+        apply TES_Var_Copy.
+        -- apply TPES_Var with (st := st); assumption.
+        -- apply usage_eqb_true. exact Husage.
+      * simpl in Hconsume.
+        destruct (sctx_consume_path Σ i []) as [Σc | err] eqn:Hconsume_path;
+          try discriminate.
+        inversion Hconsume; subst.
+        inversion Hinfer; subst.
+        eapply TES_Var_Move.
+        -- apply TPES_Var with (st := st); assumption.
+        -- intro Hu. rewrite Hu in Husage. simpl in Husage. discriminate.
+        -- exact Hconsume_path.
+    + apply andb_true_iff in Hcall as [Hcall1 Hcall2].
+      destruct (infer_core_env_state_fuel fuel' env Ω n Σ e1) as [[T1 Σ1] | err1]
+        eqn:He1; try discriminate.
+      destruct (ty_compatible_b Ω T1 t) eqn:Hcompat; try discriminate.
+      destruct (infer_core_env_state_fuel fuel' env Ω n (sctx_add i t m Σ1) e2)
+        as [[T2 Σ2] | err2] eqn:He2; try discriminate.
+      destruct (sctx_check_ok i t Σ2) eqn:Hcheck; try discriminate.
+      inversion Hinfer; subst.
+      eapply TES_Let.
+      * eapply IH; [exact Hcall1 | exact He1].
+      * exact Hcompat.
+      * eapply IH; [exact Hcall2 | exact He2].
+      * exact Hcheck.
+    + apply andb_true_iff in Hcall as [Hcall1 Hcall2].
+      destruct (infer_core_env_state_fuel fuel' env Ω n Σ e1) as [[T1 Σ1] | err1]
+        eqn:He1; try discriminate.
+      destruct (infer_core_env_state_fuel fuel' env Ω n (sctx_add i T1 m Σ1) e2)
+        as [[T2 Σ2] | err2] eqn:He2; try discriminate.
+      destruct (sctx_check_ok i T1 Σ2) eqn:Hcheck; try discriminate.
+      inversion Hinfer; subst.
+      eapply TES_LetInfer.
+      * eapply IH; [exact Hcall1 | exact He1].
+      * eapply IH; [exact Hcall2 | exact He2].
+      * exact Hcheck.
+    + destruct (lookup_fn_b i (env_fns env)) as [fdef |] eqn:Hlookup; try discriminate.
+      inversion Hinfer; subst.
+      destruct (lookup_fn_b_sound i (env_fns env) fdef Hlookup) as [Hin Hname].
+      eapply TES_Fn; eassumption.
+    + destruct (infer_place_sctx env Σ p) as [Tp | err] eqn:Hplace; try discriminate.
+      destruct (consume_place_value env Σ p Tp) as [Σ0 | err] eqn:Hconsume;
+        try discriminate.
+      unfold consume_place_value in Hconsume.
+      destruct (usage_eqb (ty_usage Tp) UUnrestricted) eqn:Husage.
+      * inversion Hconsume; subst.
+        inversion Hinfer; subst.
+        apply TES_Place_Copy.
+        -- eapply infer_place_sctx_structural_sound. exact Hplace.
+        -- apply usage_eqb_true. exact Husage.
+      * destruct (place_path p) as [[x path] |] eqn:Hpath; try discriminate.
+        destruct (sctx_consume_path Σ x path) as [Σc | err] eqn:Hconsume_path;
+          try discriminate.
+        inversion Hconsume; subst.
+        inversion Hinfer; subst.
+        eapply TES_Place_Move.
+        -- eapply infer_place_sctx_structural_sound. exact Hplace.
+        -- intro Hu. rewrite Hu in Husage. simpl in Husage. discriminate.
+        -- exact Hpath.
+        -- exact Hconsume_path.
+    + destruct (lookup_fn_b i (env_fns env)) as [fdef |] eqn:Hlookup; try discriminate.
+      rewrite infer_env_args_collect_eq in Hinfer.
+      destruct (infer_env_args_collect fuel' env Ω n Σ l) as [[arg_tys Σargs] | err]
+        eqn:Hcollect; try discriminate.
+      destruct (build_sigma (fn_lifetimes fdef) (repeat None (fn_lifetimes fdef))
+          arg_tys (fn_params fdef)) as [σ_acc |] eqn:Hbuild; try discriminate.
+      remember (apply_lt_params (finalize_subst σ_acc) (fn_params fdef)) as ps_subst.
+      destruct (check_args Ω arg_tys ps_subst) as [err |] eqn:Hcheck; try discriminate.
+      destruct (forallb (wf_lifetime_b (mk_region_ctx n)) (finalize_subst σ_acc)) eqn:Hwf;
+        try discriminate.
+      remember (apply_lt_outlives (finalize_subst σ_acc) (fn_outlives fdef)) as Ω_subst.
+      destruct (outlives_constraints_hold_b Ω Ω_subst) eqn:Hout; try discriminate.
+      inversion Hinfer; subst.
+      destruct (lookup_fn_b_sound i (env_fns env) fdef Hlookup) as [Hin Hname].
+      eapply TES_Call with (fdef := fdef) (σ := finalize_subst σ_acc).
+      * exact Hin.
+      * exact Hname.
+      * eapply infer_env_args_collect_sound.
+        -- exact Hcollect.
+        -- intros Σ0 e0 T0 Σ1 Hin_arg Hinfer_arg.
+           eapply IH.
+           ++ eapply call_exprs_in_true; eassumption.
+           ++ exact Hinfer_arg.
+        -- exact Hcheck.
+      * apply env_outlives_constraints_hold_b_sound. exact Hout.
+    + apply andb_true_iff in Hcall as [Hcallee Hargs].
+      destruct (infer_core_env_state_fuel fuel' env Ω n Σ e) as [[Tcallee Σc] | err]
+        eqn:Hcallee_infer; try discriminate.
+      rewrite infer_env_args_collect_eq in Hinfer.
+      destruct (infer_env_args_collect fuel' env Ω n Σc l) as [[arg_tys Σargs] | err]
+        eqn:Hcollect; try discriminate.
+      destruct Tcallee as [u c]; simpl in *.
+      destruct c; try discriminate.
+      * destruct (check_arg_tys Ω arg_tys l0) as [err |] eqn:Hcheck; try discriminate.
+        inversion Hinfer; subst.
+        eapply TES_CallExpr_Fn.
+        -- eapply IH; [exact Hcallee | exact Hcallee_infer].
+        -- eapply infer_env_args_collect_sound.
+           ++ exact Hcollect.
+           ++ intros Σ0 e0 T0 Σ1 Hin_arg Hinfer_arg.
+              eapply IH.
+              ** eapply call_exprs_in_true; eassumption.
+              ** exact Hinfer_arg.
+           ++ rewrite <- check_arg_tys_params_of_tys. exact Hcheck.
+      * destruct (ty_core t) eqn:Hbody; try discriminate.
+        destruct (build_bound_sigma (repeat None n0) arg_tys l0) as [σ |] eqn:Hbuild;
+          try discriminate.
+        destruct (check_arg_tys Ω arg_tys (map (open_bound_ty σ) l0)) as [err |] eqn:Hcheck;
+          try discriminate.
+        destruct (contains_lbound_ty (open_bound_ty σ t0) ||
+            contains_lbound_outlives (open_bound_outlives σ o)) eqn:Hleak;
+          try discriminate.
+        destruct (outlives_constraints_hold_b Ω (open_bound_outlives σ o)) eqn:Hout;
+          try discriminate.
+        inversion Hinfer; subst.
+        apply opened_call_no_lbound_sound in Hleak as [Hret Hbounds].
+        eapply TES_CallExpr_Forall with (σ := σ) (param_tys := l0).
+        -- eapply IH; [exact Hcallee | exact Hcallee_infer].
+        -- exact Hbody.
+        -- eapply infer_env_args_collect_sound.
+           ++ exact Hcollect.
+           ++ intros Σ0 e0 T0 Σ1 Hin_arg Hinfer_arg.
+              eapply IH.
+              ** eapply call_exprs_in_true; eassumption.
+              ** exact Hinfer_arg.
+           ++ rewrite <- check_arg_tys_params_of_tys. exact Hcheck.
+        -- exact Hret.
+        -- exact Hbounds.
+        -- apply env_outlives_constraints_hold_b_sound. exact Hout.
+    + destruct (expr_as_place e) as [p |] eqn:Hplace_expr.
+      * destruct (infer_place_sctx env Σ p) as [Tp | err] eqn:Hplace; try discriminate.
+        destruct Tp as [u c]; simpl in *.
+        destruct c; try discriminate.
+        destruct (usage_eqb (ty_usage t) UUnrestricted) eqn:Husage; try discriminate.
+        inversion Hinfer; subst.
+        eapply TES_Deref_Place.
+        -- exact Hplace_expr.
+        -- eapply infer_place_sctx_structural_sound. exact Hplace.
+        -- apply usage_eqb_true. exact Husage.
+      * destruct (infer_core_env_state_fuel fuel' env Ω n Σ e) as [[Tr Σr] | err]
+          eqn:Hr; try discriminate.
+        destruct Tr as [u c]; simpl in *.
+        destruct c; try discriminate.
+        destruct (usage_eqb (ty_usage t) UUnrestricted) eqn:Husage; try discriminate.
+        inversion Hinfer; subst.
+        eapply TES_Deref_Expr.
+        -- exact Hplace_expr.
+        -- eapply IH; [exact Hcall | exact Hr].
+        -- apply usage_eqb_true. exact Husage.
+    + destruct (infer_core_env_state_fuel fuel' env Ω n Σ e) as [[Te Σe] | err]
+        eqn:He; try discriminate.
+      inversion Hinfer; subst.
+      eapply TES_Drop. eapply IH; [exact Hcall | exact He].
+    + repeat rewrite andb_true_iff in Hcall.
+      destruct Hcall as [[Hcall1 Hcall2] Hcall3].
+      destruct (infer_core_env_state_fuel fuel' env Ω n Σ e1) as [[Tcond Σ1] | err1]
+        eqn:He1; try discriminate.
+      destruct (ty_core_eqb (ty_core Tcond) TBooleans) eqn:Hbool; try discriminate.
+      destruct (infer_core_env_state_fuel fuel' env Ω n Σ1 e2) as [[T2 Σ2] | err2]
+        eqn:He2; try discriminate.
+      destruct (infer_core_env_state_fuel fuel' env Ω n Σ1 e3) as [[T3 Σ3] | err3]
+        eqn:He3; try discriminate.
+      destruct (ty_core_eqb (ty_core T2) (ty_core T3)) eqn:Hcore; try discriminate.
+      destruct (ctx_merge (ctx_of_sctx Σ2) (ctx_of_sctx Σ3)) as [Γ4 |] eqn:Hmerge;
+        try discriminate.
+      inversion Hinfer; subst.
+      eapply TES_If.
+      * eapply IH; [exact Hcall1 | exact He1].
+      * apply ty_core_eqb_true. exact Hbool.
+      * eapply IH; [exact Hcall2 | exact He2].
+      * eapply IH; [exact Hcall3 | exact He3].
       * apply ty_core_eqb_true. exact Hcore.
       * exact Hmerge.
 Qed.
